Refactor and get rid of node counts

AvlTree/AvlTree.lean
@@ -96,10 +96,10 @@ def Zipper.go_up {α : Type} (z : Zipper α) : Option (Zipper α) :=
 #eval (Zipper.mk 2 (@AVLNode.rightie Nat 0 3 AVLNode.nil (AVLNode.balanced 2 AVLNode.nil AVLNode.nil)) (Context.root)).go_right >>= Zipper.go_up
 
 
-theorem go_left_up [BEq α] (z : Zipper α)
+theorem go_left_up (z : Zipper α)
   (h1 : some new_z = z.go_left) : new_z.go_up = z :=
   by
-  cases z with | mk n tree ctx =>
+  obtain ⟨n, tree, ctx⟩ := z
   dsimp [Zipper.go_left] at h1
   cases tree
   . simp at h1
@@ -109,9 +109,9 @@ theorem go_left_up [BEq α] (z : Zipper α)
     dsimp [Zipper.go_up]
 
 
-theorem go_right_up [BEq α] (z : Zipper α)
+theorem go_right_up (z : Zipper α)
   (h1 : some new_z = z.go_right) : new_z.go_up = z := by
-  cases z with | mk n tree ctx =>
+  obtain ⟨n, tree, ctx⟩ := z
   dsimp [Zipper.go_right] at h1
   cases tree
   . simp at h1
@@ -121,63 +121,26 @@ theorem go_right_up [BEq α] (z : Zipper α)
     dsimp [Zipper.go_up]
 
 
-def AVLNode.node_count : (AVLNode α n) → Nat
-  | .nil => 1
-  | .balanced _ l r => 1 + l.node_count + r.node_count
-  | .leftie _ l r => 1 + l.node_count + r.node_count
-  | .rightie _ l r => 1 + l.node_count + r.node_count
+def Zipper.value? : (z : Zipper α) → Option α
+  | {tree, ..} => match tree with
+    | .balanced x _ _ | .rightie x _ _ | .leftie x _ _ => x
+    | .nil => none
 
-
-theorem avl_node_count_gt_0 (t : AVLNode α n) : t.node_count > 0 := by
-  induction t
-  simp_all[AVLNode.node_count]
-  all_goals
-  rename_i _ _ t1 t2 ih1 ih2
-  simp_all[AVLNode.node_count]
-  rw [Nat.add_assoc]
-  rw [Nat.add_comm]
-  simp only [Nat.zero_lt_succ]
-
-
-theorem go_left_count_lt (z : Zipper α)
+theorem go_left_n_lt (z : Zipper α)
   (h : some lz = z.go_left)
-  : lz.tree.node_count < z.tree.node_count := by
-  cases z with | mk n tree ctx
+  : lz.n < z.n := by
+  obtain ⟨n, tree, ctx⟩ := z
   cases tree
   all_goals
   simp_all[Zipper.go_left]
-  all_goals
-  rename_i l r
-  rw[h]
-  simp_all[AVLNode.node_count]
-  rw [Nat.add_comm 1, Nat.add_assoc]
-  apply Nat.lt_add_of_pos_right
-  rw [Nat.add_comm]
-  simp only [Nat.zero_lt_succ]
 
-
-theorem go_right_count_lt (z : Zipper α)
+theorem go_right_n_lt (z : Zipper α)
   (h : some rz = z.go_right)
-  : rz.tree.node_count < z.tree.node_count := by
-  cases z with | mk n tree ctx
+  : rz.n < z.n := by
+  obtain ⟨n, tree, ctx⟩ := z
   cases tree
   all_goals
   simp_all[Zipper.go_right]
-  all_goals
-  rename_i l r
-  rw[h]
-  simp_all[AVLNode.node_count]
-  rw [Nat.add_comm]
-  simp only [Nat.zero_lt_succ]
-
-
-def Zipper.value? : (z : Zipper α) → Option α
-  | {tree, ..} => match tree with
-    | .balanced x _ _ => x
-    | .rightie x _ _ => x
-    | .leftie x _ _ => x
-    | .nil => none
-
 
 -- Zips to the element or to the Nil node where it should be inserted
 def Zipper.zip_to [Ord α] (a : α) (z : Zipper α) : Zipper α :=
@@ -186,16 +149,16 @@ def Zipper.zip_to [Ord α] (a : α) (z : Zipper α) : Zipper α :=
     | Ordering.lt => match h: z.go_left with
       | none => z
       | some lz =>
-        have : lz.tree.node_count < z.tree.node_count := by simp_all[go_left_count_lt]
+        have : lz.n < z.n := by simp_all[go_left_n_lt]
         lz.zip_to a
     | Ordering.gt => match h: z.go_right with
       | none => z
       | some rz =>
-        have : rz.tree.node_count < z.tree.node_count := by simp_all[go_right_count_lt]
+        have : rz.n < z.n := by simp_all[go_right_n_lt]
         rz.zip_to a
     | Ordering.eq => z
   else z
-termination_by z.tree.node_count
+termination_by z.n
 
 
 structure AVLTree α where
@@ -212,40 +175,41 @@ def AVLTree.from_node {α n} : (node: AVLNode α n) → AVLTree α := AVLTree.mk
 def AVLTree.unzip (t : AVLTree α) : Zipper α :=
   Zipper.mk t.n t.node Context.root
 
-def Context.node_count : (c: Context α n) → Nat
+def Context.depth : (c: Context α n) → Nat
   | .root => 0
-  | .BLC _ a b => a.node_count + b.node_count
-  | .BRC _ a b => a.node_count + b.node_count
-  | .LLC _ a b => a.node_count + b.node_count
-  | .LRC _ a b => a.node_count + b.node_count
-  | .RLC _ a b => a.node_count + b.node_count
-  | .RRC _ a b => a.node_count + b.node_count
+  | .BLC _ _ c => 1 + c.depth
+  | .BRC _ _ c => 1 + c.depth
+  | .LLC _ _ c => 1 + c.depth
+  | .LRC _ _ c => 1 + c.depth
+  | .RLC _ _ c => 1 + c.depth
+  | .RRC _ _ c => 1 + c.depth
 
 theorem zipper_ctx_nil_go_up (z : Zipper α) (h: z.ctx = Context.root)
   : z.go_up = none := by
   simp_all[Zipper.go_up]
 
-theorem zipper_go_up_ctx_node_count_lt (z : Zipper α) (h : some upper = z.go_up)
-  : upper.ctx.node_count < z.ctx.node_count := by
+theorem zipper_go_up_ctx_depth_lt (z : Zipper α) (h : some upper = z.go_up)
+  : upper.ctx.depth < z.ctx.depth := by
   obtain ⟨n, tree, ctx⟩ := z
   unfold Zipper.go_up at h
   cases ctx
-  . simp_all
+  · simp_all
   all_goals
-  rename_i val t a
-  simp_all[Context.node_count]
-  rw[h]
-  simp_all[avl_node_count_gt_0]
+    rename_i val t a
+    simp_all [Context.depth]
+    rw[h]
+    simp_all
 
-
+-- The panic here can't really be reached since we already handle the `root` case.
+-- There's probably a way to prove that it cannot happen, but I don't know how to do that yet.
 def Zipper.zip_up : (z: Zipper α) → AVLTree α
   | Zipper.mk n t .root => (AVLTree.mk n t)
   | some_z => match c: some_z.go_up with
     | some upper =>
-      have : upper.ctx.node_count < some_z.ctx.node_count := by simp_all[zipper_go_up_ctx_node_count_lt]
+      have : upper.ctx.depth < some_z.ctx.depth := by simp_all[zipper_go_up_ctx_depth_lt]
       upper.zip_up
     | none => panic! "Encountered invalid Zipper"
-termination_by z => z.ctx.node_count
+termination_by z => z.ctx.depth
 
 
 /-
@@ -361,6 +325,64 @@ def AVLNode.right_child : (AVLNode α n) → Option ((m : Nat) × AVLNode α m)
   | @AVLNode.leftie _ m _ _ r => some ⟨m, r⟩
   | @AVLNode.rightie _ m _ _ r => some ⟨m + 1, r⟩
   | .nil => none
+
+def AVLNode.node_count : (AVLNode α n) → Nat
+  | .nil => 1
+  | .balanced _ l r => 1 + l.node_count + r.node_count
+  | .leftie _ l r => 1 + l.node_count + r.node_count
+  | .rightie _ l r => 1 + l.node_count + r.node_count
+
+
+theorem avl_node_count_gt_0 (t : AVLNode α n) : t.node_count > 0 := by
+  induction t
+  simp_all[AVLNode.node_count]
+  all_goals
+  rename_i _ _ t1 t2 ih1 ih2
+  simp_all[AVLNode.node_count]
+  rw [Nat.add_assoc, Nat.add_comm]
+  simp only [Nat.zero_lt_succ]
+
+
+theorem go_left_count_lt (z : Zipper α)
+  (h : some lz = z.go_left)
+  : lz.tree.node_count < z.tree.node_count := by
+  cases z with | mk n tree ctx
+  cases tree
+  all_goals
+  simp_all[Zipper.go_left]
+  all_goals
+  rename_i l r
+  rw[h]
+  simp_all[AVLNode.node_count]
+  rw [Nat.add_comm 1, Nat.add_assoc]
+  apply Nat.lt_add_of_pos_right
+  rw [Nat.add_comm]
+  simp only [Nat.zero_lt_succ]
+
+
+theorem go_right_count_lt (z : Zipper α)
+  (h : some rz = z.go_right)
+  : rz.tree.node_count < z.tree.node_count := by
+  cases z with | mk n tree ctx
+  cases tree
+  all_goals
+  simp_all[Zipper.go_right]
+  all_goals
+  rename_i l r
+  rw[h]
+  simp_all[AVLNode.node_count]
+  rw [Nat.add_comm]
+  simp only [Nat.zero_lt_succ]
+
+
+def Context.node_count : (c: Context α n) → Nat
+  | .root => 0
+  | .BLC _ a b => a.node_count + b.node_count
+  | .BRC _ a b => a.node_count + b.node_count
+  | .LLC _ a b => a.node_count + b.node_count
+  | .LRC _ a b => a.node_count + b.node_count
+  | .RLC _ a b => a.node_count + b.node_count
+  | .RRC _ a b => a.node_count + b.node_count
 
 theorem zero_lt_node_count (t : AVLNode α n) : 0 < t.node_count := by
   induction t
